commit

AP/Util/Data/Trie/Raw.lean
@@ -4,6 +4,7 @@ namespace Trie
 
 open Std
 
+@[ext]
 structure Raw (α β : Type*) [DecidableEq α] [Hashable α] where
   inner : Raw₀ α β
   wf : inner.WF
@@ -11,12 +12,96 @@ structure Raw (α β : Type*) [DecidableEq α] [Hashable α] where
 namespace Raw
 
 variable {α β : Type*} [ha₁ : DecidableEq α] [ha₂ : Hashable α]
+variable {t t₁ t₂ t₃ : Raw α β}
 
-set_option linter.unusedVariables false in
+@[simp] instance : t.inner.WF := t.wf
+
+set_option linter.unusedVariables false
 def rec' {γ : Raw α β → Sort*}
 (motive : ∀ (val : Option β) (mp : DHashMap.Raw α (λ _ => Raw₀ α β)) wf,
-(∀ i t, mp.get? i = some t → (wf : t.WF) → γ ⟨t, wf⟩) → γ ⟨Raw₀.mk val mp, wf⟩) :
+(∀ i (t : Raw α β), mp.get? i = some t.inner → γ t) → γ ⟨Raw₀.mk val mp, wf⟩) :
 (t : Raw α β) → γ t
-| .mk (Raw₀.mk val mp) wf => motive val mp wf # λ i t h₁ wf₁ => (mk t wf₁).rec' motive
-termination_by t => t.1.depthAux
-decreasing_by exact Raw₀.depthAux_le wf h₁
+| .mk (Raw₀.mk val mp) wf => motive val mp wf # λ i t h₁ => mk t.inner t.wf |>.rec' motive
+termination_by t => t.1.depth
+decreasing_by apply Raw₀.depth_lt; exact h₁
+
+abbrev ind := @rec'
+
+@[simp]
+theorem rec'_mk {γ : Raw α β → Sort*} {val : Option β}
+{mp : DHashMap.Raw α (λ _ => Raw₀ α β)} {wf : (⟨val, mp⟩ : Raw₀ α β).WF}
+{motive : ∀ (val : Option β) (mp : DHashMap.Raw α (λ _ => Raw₀ α β)) wf,
+(∀ i (t : Raw α β), mp.get? i = some t.inner → γ t) → γ ⟨Raw₀.mk val mp, wf⟩} :
+(⟨⟨val, mp⟩, wf⟩ : Raw α β).rec' motive =
+motive val mp wf (λ _ t h => t.rec' motive) := by
+  simp [rec']
+
+def empty : Raw α β where
+  inner := ∅
+  wf := inferInstance
+
+instance : EmptyCollection # Raw α β := ⟨empty⟩
+theorem empty_def : (∅ : Raw α β) = ⟨∅, inferInstance⟩ := rfl
+
+@[simp] theorem inner_empty : (∅ : Raw α β).inner = ∅ := rfl
+
+def depth (t : Raw α β) : ℕ :=
+  t.rec' (γ := λ _ => ℕ) # λ _ mp wf f => (mp.foldWith wf.mp · 0) # λ acc i x h₂ =>
+  max acc # 1 + f i ⟨_, wf.wf_get? h₂⟩ h₂
+
+instance : SizeOf # Raw α β where
+  sizeOf := depth
+
+theorem sizeOf_def : sizeOf t = t.depth := rfl
+
+@[simp]
+theorem depth_empty : (∅ : Raw α β).depth = 0 := by
+  simp [empty_def, Raw₀.empty_def, depth]
+
+@[simp]
+theorem sizeOf_empty : sizeOf (∅ : Raw α β) = 0 :=
+  depth_empty
+
+def val (t : Raw α β) : Option β :=
+  t.inner.val
+
+@[simp]
+theorem val_mk {inner wf} : (⟨inner, wf⟩ : Raw α β).val = inner.val := rfl
+
+def get? (t : Raw α β) (k : α) : Option (Raw α β) :=
+  match h : t.inner.mp.get? k with
+  | none => none
+  | some t' => some ⟨t', t.wf.wf_get? h⟩
+
+@[simp]
+theorem get?_eq_some_iff {k t'} :
+t.get? k = some t' ↔ t.inner.mp.get? k = t'.inner := by
+  simp [get?]
+  apply Iff.intro
+  · intro a
+    split at a
+    next heq => simp_all only [reduceCtorEq]
+    next t'_1 heq =>
+      simp_all only [Option.some.injEq]
+      subst a
+      simp_all only
+  · intro a
+    split
+    next heq => simp_all only [reduceCtorEq]
+    next t'_1 heq => simp_all only [Option.some.injEq]
+
+theorem depth_eq_depth_inner : t.depth = t.inner.depth := by
+  apply t.ind
+  simp only [Raw₀.depth_mk]
+  intro val mp wf ih
+  simp only [depth, rec'_mk] at ih ⊢
+  congr
+  ext i k t' h
+  specialize ih k ⟨_, wf.wf_get? h⟩
+  rwa [ih]
+
+theorem depth_lt {k t'} (h : t.get? k = some t') : t'.depth < t.depth := by
+  simp_rw [depth_eq_depth_inner]; simp at h; exact Raw₀.depth_lt h
+
+theorem sizeOf_lt {k t'} (h : t.get? k = some t') : sizeOf t' < sizeOf t :=
+  depth_lt h
