AP/Util/Data/Trie/Trie.lean
@@ -1,10 +1,22 @@
-import AP.Util.Data.Trie.Raw
+import AP.Util.Data.Trie.Equiv
+
+variable {α β : Type*} [ha₁ : DecidableEq α] [ha₂ : Hashable α]
+
+structure Trie (α β : Type*) [DecidableEq α] [Hashable α] where
+  inner : Quotient # Trie.Raw.Setoid (α := α) (β := β)
+
+namespace Trie
 
 open Std
 
 variable {α β : Type*} [ha₁ : DecidableEq α] [ha₂ : Hashable α]
+variable {t t₁ t₂ t₃ : Trie α β}
 
--- structure Trie (α β : Type*) [DecidableEq α] [Hashable α] where
---   inner : Unit
+def empty : Trie α β :=
+  ⟨Quotient.mk _ ∅⟩
 
-namespace Trie
+instance : EmptyCollection # Trie α β := ⟨empty⟩
+theorem empty_def : (∅ : Trie α β) = empty := rfl
+
+-- def depth (t : Trie α β) : ℕ :=
+--   t.inner.lift Raw.depth # λ _ _ => Raw.Equiv.depth_eq
