AP/Util/Data/Trie/Equiv.lean
@@ -1,0 +1,98 @@
+import AP.Util.Data.Trie.Raw
+
+namespace Trie.Raw
+
+open Std
+
+variable {α β : Type*} [ha₁ : DecidableEq α] [ha₂ : Hashable α]
+variable {t t₁ t₂ t₃ : Raw α β}
+
+def Equiv (t₁ t₂ : Raw α β) : Prop :=
+  (∀ k a, t₁.get? k = some a → ∃ (b : Raw α β) (_ : t₂.get? k = some b), a.Equiv b) ∧
+  (∀ k b, t₂.get? k = some b → ∃ (a : Raw α β) (_ : t₁.get? k = some a), a.Equiv b)
+termination_by max (sizeOf t₁) (sizeOf t₂)
+decreasing_by all_goals nm h₁ h₂; have h₁ := sizeOf_lt h₁; have h₂ := sizeOf_lt h₂; omega
+
+@[refl, simp]
+theorem Equiv.refl : t.Equiv t := by
+  apply t.ind
+  intro val mp wf ih
+  unfold Equiv
+  simp only [get?_eq_some_iff, Raw₀.mp_mk, exists_prop]
+  split_ands; all_goals
+    intro k a h
+    use a, h, ih k a h
+
+@[symm]
+theorem Equiv.symm (h : t₁.Equiv t₂) : t₂.Equiv t₁ := by
+  revert t₂
+  apply t₁.ind
+  intro val mp wf ih t₂ h
+  unfold Equiv at h ⊢
+  simp only [get?_eq_some_iff, Raw₀.mp_mk, exists_prop] at h ⊢
+  rcases h with ⟨h₁, h₂⟩
+  split_ands <;> intro k a h
+  · specialize h₂ _ _ h
+    choose b h₂ h₃ using h₂
+    use b, h₂
+    apply ih _ _ h₂ h₃
+  · specialize h₁ _ _ h
+    choose b h₁ h₃ using h₁
+    use b, h₁
+    apply ih _ _ h h₃
+
+theorem Equiv.comm : t₁.Equiv t₂ ↔ t₂.Equiv t₁ :=
+  ⟨Equiv.symm, Equiv.symm⟩
+
+@[trans]
+theorem Equiv.trans (h₁ : t₁.Equiv t₂) (h₂ : t₂.Equiv t₃) : t₁.Equiv t₃ := by
+  revert t₂ t₃
+  apply t₁.ind
+  intro val mp wf ih t₂ t₃ h₁ h₂
+  unfold Equiv at h₁ h₂ ⊢
+  simp only [get?_eq_some_iff, Raw₀.mp_mk, exists_prop] at h₁ h₂ ⊢
+  rcases h₁ with ⟨h₁, h₃⟩
+  rcases h₂ with ⟨h₂, h₄⟩
+  split_ands <;> intro k a h
+  · clear h₃ h₄
+    specialize h₁ _ _ h
+    choose b h₁ h₃ using h₁
+    specialize h₂ _ _ h₁
+    choose c h₂ h₄ using h₂
+    use c, h₂
+    exact ih k a h h₃ h₄
+  · clear h₁ h₂
+    specialize h₄ _ _ h
+    choose b h₄ h₂ using h₄
+    specialize h₃ _ _ h₄
+    choose c h₃ h₁ using h₃
+    use c, h₃
+    exact ih k c h₃ h₁ h₂
+
+def Equiv.iseqv : Equivalence # Equiv (α := α) (β := β) where
+  refl _ := Equiv.refl
+  symm := Equiv.symm
+  trans := Equiv.trans
+
+instance Setoid : Setoid # Raw α β where
+  r := Equiv
+  iseqv := Equiv.iseqv
+
+namespace Equiv
+
+variable (H : t₁.Equiv t₂)
+include H
+
+-- theorem depth_eq : t₁.depth = t₂.depth := by
+--   classical
+--   revert t₂
+--   apply t₁.ind
+--   intro val mp wf ih t₂ h
+--   unfold Equiv at h
+--   simp only [get?_eq_some_iff, Raw₀.mp_mk, exists_prop] at h
+--   rcases h with ⟨h₁, h₂⟩
+--   rcases t₂ with ⟨⟨val', mp'⟩, wf'⟩
+--   unfold depth
+--   simp only [rec'_mk]
+--   simp_rw [DHashMap.Raw.foldWith_eq_foldl_toList]
+--   sorry
